src/program_proof/append_log_hocap.v
@@ -1,9 +1,12 @@
-From Perennial.goose_lang.examples Require Import append_log.
 From Perennial.goose_lang.lib Require Import encoding crash_lock.
 From Perennial.goose_lang Require Import crash_modality.
+From Perennial.goose_lang.lib Require Import into_val.
+
+From Perennial.goose_lang.examples Require Import append_log.
+
 From Perennial.program_proof Require Import proof_prelude.
 From Perennial.program_proof Require Import disk_lib.
-From Perennial.program_proof Require Import marshal_proof.
+From Perennial.goose_lang.lib Require Import slice.crash_slice.
 From Perennial.program_proof Require Import append_log_proof.
 From Perennial.goose_lang.ffi Require Import append_log_ffi.
 From Perennial.program_logic Require Import ghost_var.
